@prefix : <http://publishmydata.com/def/dataset#> .
@prefix dct: <http://purl.org/dc/terms/> .
@prefix owl: <http://www.w3.org/2002/07/owl#> .
@prefix pmd: <http://publishmydata.com/def/dataset#> .
@prefix rdf: <http://www.w3.org/1999/02/22-rdf-syntax-ns#> .
@prefix xml: <http://www.w3.org/XML/1998/namespace> .
@prefix xsd: <http://www.w3.org/2001/XMLSchema#> .
@prefix rdfs: <http://www.w3.org/2000/01/rdf-schema#> .
@base <http://publishmydata.com/def/dataset> .

<http://publishmydata.com/def/dataset> rdf:type owl:Ontology ;
                                        dct:modified "2014-07-29"^^xsd:date ,
                                                     "2018-11-29"^^xsd:date ;
                                        rdfs:label "PublishMyData Ontology" ;
                                        dct:created "2014-07-29"^^xsd:date ;
                                        rdfs:comment "Ontology of terms used by PublishMyData." ;
                                        dct:title "PublishMyData Ontology" .

#################################################################
#    Annotation properties
#################################################################

###  http://publishmydata.com/def/dataset#contactEmail
pmd:contactEmail rdf:type owl:AnnotationProperty ;
                 rdfs:comment "An email address where users of a dataset can send comments or questions.  The value should be a mailto: URL" ;
                 rdfs:isDefinedBy <http://publishmydata.com/def/dataset> ;
                 rdfs:label "Contact email" ;
                 rdfs:domain pmd:Dataset .


###  http://publishmydata.com/def/dataset#graph
pmd:graph rdf:type owl:AnnotationProperty ;
          rdfs:comment "Relates a dataset to the URL of the named graph that holds the contents of that dataset." ;
          rdfs:isDefinedBy <http://publishmydata.com/def/dataset> ;
          rdfs:label "Graph" ;
          rdfs:domain pmd:Dataset .


#################################################################
#    Datatypes
#################################################################

###  http://www.w3.org/2001/XMLSchema#date
xsd:date rdf:type rdfs:Datatype .


#################################################################
#    Data properties
#################################################################

###  http://publishmydata.com/def/dataset#nextUpdateDue
pmd:nextUpdateDue rdf:type owl:DatatypeProperty ;
                  rdfs:subPropertyOf pmd:releaseDate ;
                  rdfs:range xsd:string ;
                  rdfs:comment "A possibly approximate estimate of when the next expected update to a resource will be.  This property may be updated and revised with new values, representing either refined estimates of the next release or with a new value for a new release entirely."^^xsd:string ;
                  rdfs:label "Next update due"^^xsd:string .


###  http://publishmydata.com/def/dataset#releaseDate
pmd:releaseDate rdf:type owl:DatatypeProperty ;
                rdfs:subPropertyOf owl:topDataProperty ;
                rdfs:comment "A release date, can be any time in the past, present or future.  Or an approximation of a release date, e.g. \"some time around May\"."^^xsd:string ;
                rdfs:label "Release date"^^xsd:string .


###  http://publishmydata.com/def/dataset#updateDueOn
pmd:updateDueOn rdf:type owl:DatatypeProperty ;
                rdfs:subPropertyOf pmd:releaseDate ;
                rdfs:range xsd:date ;
                rdfs:comment "The expected date; past, present or future, of an update to a resource."^^xsd:string ;
                rdfs:label "Update due on"^^xsd:string .


#################################################################
#    Classes
#################################################################

###  http://publishmydata.com/def/dataset#Dataset
pmd:Dataset rdf:type owl:Class ;
            rdfs:comment "A dataset suitable for use in the PublishMyData software platform." ;
            rdfs:isDefinedBy <http://publishmydata.com/def/dataset> ;
            rdfs:label "Dataset" .


###  http://publishmydata.com/def/dataset#LinkedDataset
pmd:LinkedDataset rdf:type owl:Class ;
                  rdfs:subClassOf pmd:Dataset ;
                  rdfs:comment "A dataset containing linked-data suitable for use in the PublishMyData software platform." ;
                  rdfs:isDefinedBy <http://publishmydata.com/def/dataset> ;
                  rdfs:label "Linked Dataset" .


###  Generated by the OWL API (version 4.2.8.20170104-2310) https://github.com/owlcs/owlapi
