@prefix rdf: <http://www.w3.org/1999/02/22-rdf-syntax-ns#> .
@prefix rdfs: <http://www.w3.org/2000/01/rdf-schema#> .
@prefix owl: <http://www.w3.org/2002/07/owl#> .
@prefix geo: <http://www.opengis.net/ont/geosparql#> .
@prefix pmdgeo: <http://publishmydata.com/def/pmdgeo/> .
@prefix xsd: <http://www.w3.org/2001/XMLSchema#> .

<http://publishmydata.com/def/pmdgeo> rdf:type  owl:Ontology;
  rdfs:label "Publish My Data Geometry Ontology";
  rdfs:comment "The PMD Geometry Ontology extends OGC GeoSPARQL to support GeoJSON, and OS spatial relations to support string representations of grid references.";
  rdfs:seeAlso <http://www.opengis.net/ont/geosparql>;
  .

pmdgeo:asGeoJSON rdfs:subPropertyOf geo:hasSerialization;
  rdfs:label "asGeoJSON";
  rdfs:comment "The GeoJSON serialisation of a geometry";
  rdfs:domain geo:Geometry;
  rdfs:range pmdgeo:geoJsonLiteral;
  rdfs:isDefinedBy <http://publishmydata.com/def/pmdgeo>;
  rdfs:seeAlso <https://geojson.org>
  .

pmdgeo:geoJsonLiteral a rdfs:Datatype;
  rdfs:label "GeoJSON Literal";
  rdfs:comment "A GeoJSON encoding of geographic data structure using the IETF RFC 7946 standard";
  rdfs:isDefinedBy <http://publishmydata.com/def/pmdgeo>;
  rdfs:seeAlso <https://tools.ietf.org/html/rfc7946>;
  .

pmdgeo:simplificationPercent a rdf:Property;
  rdfs:label "Simplification Percent";
  rdfs:comment "The percentage simplification that was applied to the source to derive this geometry. 100 means no simplification.";
  rdfs:domain geo:Geometry;
  rdfs:range xsd:integer;
  rdfs:isDefinedBy <http://publishmydata.com/def/pmdgeo>;
  .

<http://publishmydata.com/def/pmdgeo/spatialrelations/fourFigureGridReference> a rdf:Property;
  rdfs:label "Ordnance Survey 4 Figure Grid Reference";
  rdfs:comment "A string representation of an Ordnance Survey 4 figure grid reference (e.g. SJ8398) which denotes a 1km x 1km square.";
  rdfs:isDefinedBy <http://publishmydata.com/def/pmdgeo>;
  rdfs:seeAlso <http://data.ordnancesurvey.co.uk/ontology/spatialrelations/oneKMGridReference>;
  .

<http://publishmydata.com/def/pmdgeo/spatialrelations/sixFigureGridReference> a rdf:Property;
  rdfs:label "Ordnance Survey 6 Figure Grid Reference";
  rdfs:comment "A string representation of an Ordnance Survey 6 figure grid reference (e.g. SJ838980) which denotes a 100m x 100m square.";
  rdfs:isDefinedBy <http://publishmydata.com/def/pmdgeo>;
  .

<http://publishmydata.com/def/pmdgeo/spatialrelations/eightFigureGridReference> a rdf:Property;
  rdfs:label "Ordnance Survey 8 Figure Grid Reference";
  rdfs:comment "A string representation of an Ordnance Survey 8 figure grid reference (e.g. SJ83819805) which denotes a 10m x 10m square.";
  rdfs:isDefinedBy <http://publishmydata.com/def/pmdgeo>;
  .

<http://publishmydata.com/def/pmdgeo/spatialrelations/tenFigureGridReference> a rdf:Property;
  rdfs:label "Ordnance Survey 10 Figure Grid Reference";
  rdfs:comment "A string representation of an Ordnance Survey 10 figure grid reference (e.g. SJ8381998052) which denotes a 1m x 1m square.";
  rdfs:isDefinedBy <http://publishmydata.com/def/pmdgeo>;
  .
